format update

otbn_model/spec/def.dfy
@@ -79,9 +79,8 @@ datatype ins256 =
 
 datatype codes = CNil | va_CCons(hd:code, tl:codes)
 
-// datatype cmp = Eq | Ne | Gt | Ge | Lt | Le
-// datatype whileCond = WhileCond(cmp:cmp, r:Reg32, c:uint32)
-datatype whileCond = WhileCond(r:Reg32)
+datatype cmp = Eq | Ne | Gt | Ge | Lt | Le
+datatype whileCond = WhileCond(cmp:cmp, r:Reg32, c:uint32)
 
 datatype code =
 | Ins32(ins:ins32)
@@ -89,18 +88,18 @@ datatype code =
 | Block(block:codes)
 | While(whileCond:whileCond, whileBody:code)
 
-datatype flagGroup = flagGroup(cf:bool, msb:bool, lsb:bool, zero:bool)
-datatype Flags = Flags(fg0:flagGroup, fg1:flagGroup)
+datatype FlagsGroup = FlagsGroup(cf:bool, msb:bool, lsb:bool, zero:bool)
+datatype Flags = Flags(fg0:FlagsGroup, fg1:FlagsGroup)
 
 datatype state = state(
-    xregs: map<Reg32, uint32>,
-    wregs: map<Reg256, uint256>,
+    xregs: map<Reg32, uint32>, // 32-bit registers
+    wregs: map<Reg256, uint256>, // 256-bit registers
     flags: Flags,
-    lstack: seq<uint32>,
+    lstack: seq<nat>,
     ok: bool)
 
-function fst(t:(uint256, flagGroup)) : uint256 { t.0 }
-function snd(t:(uint256, flagGroup)) : flagGroup { t.1 }
+function fst(t:(uint256, FlagsGroup)) : uint256 { t.0 }
+function snd(t:(uint256, FlagsGroup)) : FlagsGroup { t.1 }
 
 predicate IsUInt32(i:int) { 0 <= i < 0x1_0000_0000 }
 predicate IsUInt256(i:int) { 0 <= i < 0x1_00000000_00000000_00000000_00000000_00000000_00000000_00000000_00000000 }
@@ -193,33 +192,39 @@ predicate evalBlock(block:codes, s:state, r:state)
         exists r':state :: evalCode(block.hd, s, r') && evalBlock(block.tl, r', r)
 }
 
-predicate loopStackNoneEmpty(s: state)
+function evalCmp(c:cmp, i1:uint32, i2:uint32):bool
 {
-    |s.lstack| != 0
+    match c
+        case Eq => i1 == i2
+        case Ne => i1 != i2
+        case Gt => i1 > i2
+        case Ge => i1 >= i2
+        case Lt => i1 < i2
+        case Le => i1 <= i2
 }
 
-function evalWhileCond(s: state, wc: whileCond): bool
+function evalWhileCond(s:state, wc:whileCond):bool
     requires ValidSourceRegister32(s, wc.r);
-    requires loopStackNoneEmpty(s);
+    requires IsUInt32(wc.c);
 {
-    s.lstack[0] != eval_reg32(s, wc.r)  
+    evalCmp(wc.cmp, eval_reg32(s, wc.r), wc.c)
 }
 
-predicate branchRelation(s:state, r:state, cond:bool)
-    requires loopStackNoneEmpty(s);
+function {:axiom} updateFlagsUsingCondition(flags:Flags, cond:bool) : Flags
+
+predicate branchRelation(s:state, s':state, cond:bool)
 {
-    r == s.(lstack := s.lstack[1..])
+    s' == s.(flags := updateFlagsUsingCondition(s.flags, cond))
 }
 
 predicate evalWhile(wc:whileCond, c:code, n:nat, s:state, r:state)
     decreases c, n
 {
-    if s.ok && ValidSourceRegister32(s, wc.r) && loopStackNoneEmpty(s) then
+    if s.ok && ValidSourceRegister32(s, wc.r) && IsUInt32(wc.c) then
         if n == 0 then
             !evalWhileCond(s, wc) && branchRelation(s, r, false)
         else
-            exists loop_start: state, loop_end: state :: 
-            evalWhileCond(s, wc)
+            exists loop_start:state, loop_end:state :: evalWhileCond(s, wc)
             && branchRelation(s, loop_start, true)
             && evalCode(c, loop_start, loop_end)
             && evalWhile(wc, c, n - 1, loop_end, r)
@@ -235,10 +240,10 @@ predicate evalCode(c:code, s:state, r:state)
         case Ins256(ins) => evalIns256(ins, s, r)
         case Block(block) => evalBlock(block, s, r)
         //case IfElse(cond, ifT, ifF) => evalIfElse(cond, ifT, ifF, s, r)
-        case While(cond, body) => exists n: nat :: evalWhile(cond, body, n, s, r)
+        case While(cond, body) => exists n:nat :: evalWhile(cond, body, n, s, r)
 }
 
-function get_flags_group(fg:bool, flags:Flags) : flagGroup { if fg then flags.fg1 else flags.fg0 }
+function get_flags_group(fg:bool, flags:Flags) : FlagsGroup { if fg then flags.fg1 else flags.fg0 }
 
 function get_flag(fg:bool, flag:int, flags:Flags) : bool
     requires 0 <= flag <= 4;
@@ -249,23 +254,23 @@ function get_flag(fg:bool, flag:int, flags:Flags) : bool
     get_flags_group(fg, flags).zero
 }
 
-function update_fg(b:bool, f:Flags, fg:flagGroup) : Flags { if b then f.(fg1 := fg) else f.(fg0 := fg) }
+function update_fg(b:bool, f:Flags, fg:FlagsGroup) : Flags { if b then f.(fg1 := fg) else f.(fg0 := fg) }
 
-function cf(flags_group:flagGroup) : bool { flags_group.cf }
+function cf(flags_group:FlagsGroup) : bool { flags_group.cf }
 
-function bn_add(x: uint256, y: uint256, st: bool, sb: uint32) : (uint256, flagGroup)
+function bn_add(x: uint256, y: uint256, st: bool, sb: uint32) : (uint256, FlagsGroup)
     requires sb < 32;
 {
     bn_add_carray(x, uint256_sb(y, st, sb), false)
 }
 
-function bn_addc(x: uint256, y: uint256, st: bool, sb: uint32, flags_group:flagGroup) : (uint256, flagGroup)
+function bn_addc(x: uint256, y: uint256, st: bool, sb: uint32, flags_group:FlagsGroup) : (uint256, FlagsGroup)
     requires sb < 32;
 {
     bn_add_carray(x, uint256_sb(y, st, sb), cf(flags_group))
 }
 
-function bn_addi(x: uint256, imm: uint256) : (uint256, flagGroup)
+function bn_addi(x: uint256, imm: uint256) : (uint256, FlagsGroup)
     requires imm < 1024;
 {
     bn_add_carray(x, imm, false)
@@ -277,33 +282,33 @@ function bn_addm(x: uint256, y: uint256, mod: uint256) : uint256
     if sum >= mod then sum - mod else sum
 }
 
-function bn_sub(x: uint256, y: uint256, st: bool, sb: uint32) : (uint256, flagGroup)
+function bn_sub(x: uint256, y: uint256, st: bool, sb: uint32) : (uint256, FlagsGroup)
     requires sb < 32;
 {
     var diff :int := x - uint256_sb(y, st, sb);
     // FIXME: figure out the flags
-    var fg := flagGroup(false, false, false, diff == 0);
+    var fg := FlagsGroup(false, false, false, diff == 0);
     (diff % BASE_256, fg)
 }
 
-function bn_subb(x: uint256, y: uint256, st: bool, sb :uint32, flags_group: flagGroup) : (uint256, flagGroup)
+function bn_subb(x: uint256, y: uint256, st: bool, sb :uint32, flags_group: FlagsGroup) : (uint256, FlagsGroup)
     requires sb < 32;
 {
     // FIXME: double check this
     var cf := if cf(flags_group) then 1 else 0;
     var diff :int := x - uint256_sb(y, st, sb) - cf;
-    var fg := flagGroup(false, false, false, diff == 0);
+    var fg := FlagsGroup(false, false, false, diff == 0);
     (diff % BASE_256, fg)
 }
 
-function bn_subbi(x: uint256, imm: uint256) : (uint256, flagGroup)
+function bn_subbi(x: uint256, imm: uint256) : (uint256, FlagsGroup)
     requires imm < 1024;
     // requires imm < x; //TODO: Is this true?
 {
     // FIXME: double check this
     var diff :int := x - imm;
     // FIXME: figure out the flags
-    var fg := flagGroup(false, false, false, diff == 0);
+    var fg := FlagsGroup(false, false, false, diff == 0);
     (diff % BASE_256, fg)
 }
 
@@ -315,11 +320,11 @@ function bn_subm(x: uint256, y: uint256, wmod: uint256) : uint256
     if result >= wmod then (result as bv256 - wmod as bv256) as uint256 else result
 }
 
-function bn_add_carray(a: uint256, b: uint256, carry_in: bool) : (uint256, flagGroup)
+function bn_add_carray(a: uint256, b: uint256, carry_in: bool) : (uint256, FlagsGroup)
 {
     var sum :int := a + b + if carry_in then 1 else 0;
     // FIXME: get MSB and LSM
-    var fg := flagGroup(sum >= BASE_256, false, false, sum == 0);
+    var fg := FlagsGroup(sum >= BASE_256, false, false, sum == 0);
     (sum % BASE_256, fg)
 }
 
